Reverted previous commit that was accidental. I only wanted to store the patch for later reference (it is in patches/bvector.diff). Also in this commit is substitution on coinductive terms.

Substitution.v
@@ -1,4 +1,3 @@
-Require Import Prelims.
 Require Export FiniteTerm.
 Require Export Term.
 Require Import TermEquality.
@@ -25,20 +24,72 @@ Definition empty_substitution (x : X) : term := Var x.
 Fixpoint substitute (sigma : substitution) (t : fterm) {struct t} : term :=
   match t with
   | FVar x      => sigma x
-  | FFun f args => Fun f (Vmap (substitute sigma) args)
+  | FFun f args => Fun f (vmap (substitute sigma) args)
   end.
 
 (* Applying the empty substitution to a finite term gives the trivial infinite term image *)
+(* The only reason we cannot prove coq-equality here is equality on vectors *)
 Lemma empty_substitution_is_trivial :
   forall (t : fterm), substitute empty_substitution t [~] t.
 Proof.
-admit.
-(*
 induction t.
 apply term_bis_refl.
 constructor.
 assumption.
-*)
+Qed.
+
+(* TODO: with the recursive vectors we can also define this as a cofixpoint on
+   (non-finite) terms. Below are some additional lemmas for reassurance. *)
+CoFixpoint substitute' (sigma : substitution) (t : term) : term :=
+  match t with
+  | Var x      => sigma x
+  | Fun f args => Fun f (vmap (substitute' sigma) args)
+  end.
+
+(* Take apart a coinductive term up to depth 1 and put it back together *)
+Definition peek (t : term) : term :=
+  match t with
+  | Var x      => Var x
+  | Fun f args => Fun f args
+  end.
+
+Theorem peek_eq : forall (t : term), t = peek t.
+  destruct t; reflexivity.
+Qed.
+
+(* Applying the empty substitution to a finite term gives the trivial infinite term image *)
+Lemma empty_substitution_is_trivial' :
+  forall (t : term), substitute' empty_substitution t [~] t.
+Proof.
+cofix IH.
+destruct t.
+rewrite (peek_eq (substitute' empty_substitution (Var v))).
+apply term_bis_refl.
+rewrite (peek_eq (substitute' empty_substitution (Fun f v))).
+simpl.
+constructor.
+intro i.
+unfold vmap.
+apply IH.
+Qed.
+
+(* the following can be proved for coq-equality were it not that
+   we cannot equate (vmap finite_term_as_term v) and v *)
+Lemma substitutions_related :
+  forall (s : substitution) (t : fterm), substitute s t [~] substitute' s t.
+Proof.
+induction t.
+simpl.
+rewrite (peek_eq (substitute' s (Var v))).
+simpl.
+destruct (s v); apply term_bis_refl.
+simpl.
+rewrite (peek_eq (substitute' s (Fun f (vmap (@finite_term_as_term F X) v)))).
+simpl.
+constructor.
+intro i.
+unfold vmap.
+apply H.
 Qed.
 
 End Substitution.
